examples-c/schorr-waite/coq/BinTree.v
@@ -36,6 +36,17 @@ Inductive reachable (a: alloc_table) (l: memory pointer)(r: memory pointer) : po
         	valid a p1 ->
         	  reachable a l r (acc r p1)  p2 -> reachable a l r p1 p2.
    
+Inductive unmarked_reachable (a: alloc_table) (l: memory pointer)(m:memory Z)(r: memory pointer) : pointer ->  pointer -> Prop :=
+  | Path_unmarked_null : forall p:pointer, (acc m p) = 0 ->unmarked_reachable a l m r p  p
+  | Path_unmarked_left :
+      forall p1 p2:pointer,
+        valid a p1 ->
+          unmarked_reachable a l m r (acc l p1) p2-> (acc m p1) = 0 -> unmarked_reachable a l m r p1  p2
+  | Path_unmarked_right :
+      	forall p1 p2:pointer,
+        	valid a p1 ->
+        	  unmarked_reachable a l m r (acc r p1)  p2 -> (acc m p1) = 0-> unmarked_reachable a l m r p1 p2.
+
 Inductive stkOk   (c:memory Z) (l: memory pointer)(r: memory pointer) 
 (iL : memory pointer)(iR: memory pointer) : pointer ->  list pointer -> Prop :=
 | stkOk_nil : forall t : pointer, stkOk  c l r iL iR t nil 
@@ -47,11 +58,30 @@ stkOk  c l r iL iR t (cons p stk).
 Inductive clr_list (a: alloc_table)  (c:memory Z) (l: memory pointer)
 (r: memory pointer) : pointer ->list pointer-> Prop :=
 | clr_list_nil : forall t : pointer , clr_list a c l r t nil 
-| clr_list_cons : forall t : pointer, forall p : pointer, forall stack : list pointer, 
-clr_list a c l r p stack -> (p = if Zneq_bool (acc c t) 0 then (acc r t) else (acc l t)) ->
-clr_list a c l r t (cons p stack).
+| clr_list_cons : 
+   forall t : pointer, forall p : pointer, forall stack : list pointer, 
+     clr_list a c l r p stack -> valid a t ->
+       (p = if Zneq_bool (acc c t) 0 then (acc r t) else (acc l t)) ->
+          clr_list a c l r t (cons p stack).
 
 Inductive all_in_list (m:memory Z) : list pointer -> Prop :=
 | all_in_list_nil : all_in_list m nil 
 | all_in_list_cons : forall l : list pointer, forall t : pointer,
 all_in_list m l -> (acc m t) <> 0 -> all_in_list m (cons t l).
+
+Lemma reachable_unchanged:forall l0 r0 l r : memory pointer,
+(forall x : pointer, (acc r0 x) = (acc r x) /\ (acc l0 x)= (acc l x)) -> 
+forall a :alloc_table ,forall root x : pointer , reachable a l0 r0 root x -> reachable a l r root x. 
+intros.
+induction H0.
+constructor.
+apply Path_left;auto.
+replace (acc l p1) with (acc l0 p1).
+auto.
+generalize (H p1);intuition.
+apply Path_right;auto.
+replace (acc r p1) with (acc r0 p1).
+auto.
+generalize (H p1);intuition.
+Qed.
+
